add(FirstOrder): forcing part.1 (#604)

Foundation/Logic/ForcingRelation.lean
@@ -7,17 +7,22 @@ class ForcingRelation (W : Type*) (F : outParam Type*) where
 
 infix:45 " ⊩ " => ForcingRelation.Forces
 
+class ForcingExists (W : Type*) (α : outParam Type*) where
+  Forces : W → α → Prop
+
+infix:45 " ⊩↓ " => ForcingExists.Forces
+
 namespace ForcingRelation
 
 variable {W : Type*} {F : Type*} [ForcingRelation W F] [LogicalConnective F]
 
-abbrev NotForces (w : W) (φ : F) : Prop := ¬ w ⊩ φ
+abbrev NotForces (w : W) (φ : F) : Prop := ¬w ⊩ φ
 
 infix:45 " ⊮ " => NotForces
 
 variable (W)
 
-class IntuitionisticKripke (R : outParam (W → W → Prop)) where
+class IntKripke (R : outParam (W → W → Prop)) where
   verum (w : W) : w ⊩ ⊤
   falsum (w : W) : w ⊮ ⊥
   and (w : W) : w ⊩ φ ⋏ ψ ↔ w ⊩ φ ∧ w ⊩ ψ
@@ -25,9 +30,50 @@ class IntuitionisticKripke (R : outParam (W → W → Prop)) where
   not (w : W) : w ⊩ ∼φ ↔ (∀ v, R w v → v ⊮ φ)
   imply (w : W) : w ⊩ φ ➝ ψ ↔ (∀ v, R w v → v ⊩ φ → v ⊩ ψ)
 
-attribute [simp, grind] IntuitionisticKripke.verum IntuitionisticKripke.falsum IntuitionisticKripke.and IntuitionisticKripke.or
-attribute [grind] IntuitionisticKripke.imply IntuitionisticKripke.not
+variable {W}
+
+attribute [simp, grind]
+  IntKripke.verum IntKripke.falsum IntKripke.and
+  IntKripke.or IntKripke.imply IntKripke.not
+attribute [grind]
+  IntKripke.imply IntKripke.not
+
+namespace IntKripke
+
+variable {R : W → W → Prop} [IntKripke W R]
+
+end IntKripke
 
 end ForcingRelation
+
+class WeakForcingRelation (W : Type*) (F : outParam Type*) where
+  Forces : W → F → Prop
+
+infix:45 " ⊩ᶜ " => WeakForcingRelation.Forces
+namespace WeakForcingRelation
+
+variable {W : Type*} {F : Type*} [WeakForcingRelation W F] [LogicalConnective F]
+
+abbrev NotForces (w : W) (φ : F) : Prop := ¬w ⊩ᶜ φ
+
+infix:45 " ⊮ᶜ " => NotForces
+
+variable (W)
+
+class ClassicalKripke (R : outParam (W → W → Prop)) where
+  verum (w : W) : w ⊩ᶜ ⊤
+  falsum (w : W) : w ⊮ᶜ ⊥
+  and (w : W) : w ⊩ᶜ φ ⋏ ψ ↔ w ⊩ᶜ φ ∧ w ⊩ᶜ ψ
+  or (w : W) : w ⊩ᶜ φ ⋎ ψ ↔ ∀ v, R w v → ∃ x, R v x ∧ (x ⊩ᶜ φ ∨ x ⊩ᶜ ψ)
+  not (w : W) : w ⊩ᶜ ∼φ ↔ (∀ v, R w v → v ⊮ᶜ φ)
+  imply (w : W) : w ⊩ᶜ φ ➝ ψ ↔ (∀ v, R w v → v ⊩ᶜ φ → v ⊩ᶜ ψ)
+
+attribute [simp, grind]
+  ClassicalKripke.verum ClassicalKripke.falsum ClassicalKripke.and
+  ClassicalKripke.or ClassicalKripke.imply ClassicalKripke.not
+attribute [grind]
+  ClassicalKripke.imply ClassicalKripke.not
+
+end WeakForcingRelation
 
 end LO
