Foundation/FirstOrder/Intuitionistic/Rew.lean
@@ -1,4 +1,4 @@
-import Foundation.IntFO.Basic.Formula
+import Foundation.FirstOrder.Intuitionistic.Formula
 
 namespace LO.FirstOrder
 
