Foundation/FirstOrder/Kripke/Basic.lean
@@ -1,0 +1,82 @@
+import Foundation.Vorspiel.Preorder
+import Foundation.FirstOrder.Basic
+import Foundation.Logic.Predicate.Relational
+import Foundation.Logic.ForcingRelation
+import Mathlib.Order.PFilter
+
+namespace LO.FirstOrder
+
+/-- Kripke model for relational first-order language -/
+structure KripkeModel (L : Language) [L.Relational] where
+  Condition : Type*
+  [preorder : Preorder Condition]
+  Name : Type*
+  Domain : Condition → Set Name
+  domain_nonempty : ∀ w, ∃ x, x ∈ Domain w
+  domain_antimonotone : w ≥ v → Domain w ⊆ Domain v
+  Rel (w : Condition) {k : ℕ} (R : L.Rel k) : (Fin k → Name) → Prop
+  rel_monotone : Rel w R t → ∀ v ≤ w, Rel v R t
+
+variable (L : Language) [L.Relational]
+
+instance : CoeSort (KripkeModel L) (Type _) := ⟨fun 𝓚 ↦ 𝓚.Condition⟩
+
+instance (𝓚 : KripkeModel L) : CoeSort 𝓚.Condition (Type _) := ⟨fun w ↦ 𝓚.Domain w⟩
+
+instance (𝓚 : KripkeModel L) : Preorder 𝓚.Condition := 𝓚.preorder
+
+instance (𝓚 : KripkeModel L) : ForcingExists 𝓚 𝓚.Name := ⟨fun p x ↦ x ∈ 𝓚.Domain p⟩
+
+variable {L}
+
+namespace KripkeModel
+
+variable (𝓚 : KripkeModel L)
+
+lemma domain_nonempty' (p : 𝓚) : ∃ x, p ⊩↓ x := 𝓚.domain_nonempty p
+
+lemma domain_antimonotone' {p : 𝓚} : p ⊩↓ x → ∀ q ≤ p, q ⊩↓ x := fun hx _ h ↦
+  𝓚.domain_antimonotone h hx
+
+@[simp] lemma domain_forcesExists {p : 𝓚} (x : p) : p ⊩↓ x.val := x.prop
+
+abbrev Filter : Type _ := Order.PFilter 𝓚
+
+variable {𝓚}
+
+namespace Filter
+
+/-- A domain of filter `F` -/
+@[ext] structure Domain (F : 𝓚.Filter) where
+  val : 𝓚.Name
+  mem_filter : ∃ p ∈ F, p ⊩↓ val
+
+attribute [coe] Domain.val
+
+variable (F : 𝓚.Filter)
+
+instance : CoeOut F.Domain 𝓚.Name := ⟨fun x ↦ x.val⟩
+
+lemma finite_colimit [Fintype ι] (p : ι → 𝓚) (hp : ∀ i, p i ∈ F) : ∃ q ∈ F, ∀ i, q ≤ p i :=
+  DirectedOn.fintype_colimit transitive_ge (Order.PFilter.nonempty F) F.directed p hp
+
+lemma finite_colimit_domain [Fintype ι] (v : ι → F.Domain) :
+    ∃ q ∈ F, ∀ i, q ⊩↓ ↑(v i) := by
+  have : ∀ i, ∃ p ∈ F, p ⊩↓ ↑(v i) := fun i ↦ (v i).mem_filter
+  choose p hp using this
+  have : ∃ q ∈ F, ∀ i, q ≤ p i := F.finite_colimit p fun i ↦ (hp i).1
+  rcases this with ⟨q, hq, hqp⟩
+  refine ⟨q, hq, fun i ↦ 𝓚.domain_antimonotone (hqp i) (hp i).2⟩
+
+instance Str : Structure L F.Domain where
+  func _ f _ := IsEmpty.elim' inferInstance f
+  rel _ R v := ∀ p ∈ F, (∀ i, p ⊩↓ ↑(v i)) → 𝓚.Rel p R fun i ↦ v i
+
+@[simp] lemma Str.rel_iff {k : ℕ} (R : L.Rel k) (v : Fin k → F.Domain) :
+    F.Str.rel R v ↔ ∀ p ∈ F, (∀ i, p ⊩↓ ↑(v i)) → 𝓚.Rel p R fun i ↦ v i := by rfl
+
+end Filter
+
+end KripkeModel
+
+end LO.FirstOrder
