Foundation/FirstOrder/Kripke/WeakForcing.lean
@@ -1,0 +1,264 @@
+import Foundation.FirstOrder.Kripke.Intuitionistic
+import Foundation.FirstOrder.NegationTranslation.GoedelGentzen
+
+/-! # Weak forcing
+
+Main reference: Jeremy Avigad, "Forcing in proof theory"
+-/
+
+namespace LO.FirstOrder.KripkeModel
+
+variable {L : Language} [L.Relational] {ℙ : KripkeModel L}
+
+def WeaklyForces (p : ℙ) (bv : Fin n → ℙ.Name) (fv : ξ → ℙ.Name) (φ : Semiformula L ξ n) : Prop := ℙ.Forces p bv fv φᴺ
+
+local notation:45 p " ⊩[" bv "|" fv "] " φ:46 => WeaklyForces p bv fv φ
+
+@[simp] lemma exists_le {α : Type*} [Preorder α] (a : α) : ∃ x, x ≤ a := ⟨a, by rfl⟩
+namespace WeaklyForces
+
+variable {bv : Fin n → ℙ.Name} {fv : ξ → ℙ.Name}
+
+@[simp] lemma rel {R : L.Rel k} {t : Fin k → Semiterm L ξ n} :
+    p ⊩[bv|fv] Semiformula.rel R t ↔ ∀ q ≤ p, ∃ r ≤ q, ℙ.Rel r R fun i ↦ (t i).relationalVal bv fv := by simp [WeaklyForces]
+
+@[simp] lemma nrel {R : L.Rel k} {t : Fin k → Semiterm L ξ n} :
+    p ⊩[bv|fv] Semiformula.nrel R t ↔ ∀ q ≤ p, ¬ℙ.Rel q R fun i ↦ (t i).relationalVal bv fv := by simp [WeaklyForces]
+
+@[simp] lemma verum : p ⊩[bv|fv] (⊤ : Semiformula L ξ n) := by simp [WeaklyForces]
+
+@[simp] lemma falsum : ¬p ⊩[bv|fv] (⊥ : Semiformula L ξ n) := by rintro ⟨⟩
+
+@[simp] lemma and {φ ψ : Semiformula L ξ n} :
+    p ⊩[bv|fv] φ ⋏ ψ ↔ p ⊩[bv|fv] φ ∧ p ⊩[bv|fv] ψ := by simp [WeaklyForces]
+
+@[simp] lemma or {φ ψ : Semiformula L ξ n} :
+    p ⊩[bv|fv] φ ⋎ ψ ↔ ∀ q ≤ p, ∃ r ≤ q, r ⊩[bv|fv] φ ∨ r ⊩[bv|fv] ψ := by
+  suffices
+      (∀ q ≤ p, (∃ r ≤ q, Forces r bv fv φᴺ) ∨ ∃ r ≤ q, Forces r bv fv ψᴺ) ↔
+      ∀ q ≤ p, ∃ r ≤ q, Forces r bv fv φᴺ ∨ Forces r bv fv ψᴺ by
+    simpa [WeaklyForces, -not_and, not_and_or]
+  grind
+
+@[simp] lemma all {φ : Semiformula L ξ (n + 1)} :
+    p ⊩[bv|fv] ∀' φ ↔ ∀ q ≤ p, ∀ x : q, WeaklyForces q (x :> bv) fv φ := by simp [WeaklyForces]
+
+@[simp] lemma ex {φ : Semiformula L ξ (n + 1)} :
+    p ⊩[bv|fv] ∃' φ ↔ ∀ q ≤ p, ∃ r ≤ q, ∃ x : r, r ⊩[x :> bv|fv] φ := by
+  suffices
+      (∀ q ≤ p, ∃ r ≤ q, ∃ x ∈ ℙ.Domain r, ∃ s ≤ r, s ⊩[x :> bv|fv] φ) ↔
+      (∀ q ≤ p, ∃ r ≤ q, ∃ x ∈ ℙ.Domain r, r ⊩[x :> bv|fv] φ) by
+    simpa [WeaklyForces]
+  constructor
+  · intro h q hqp
+    rcases h q hqp with ⟨r, hrq, x, hx, s, hsr, H⟩
+    exact ⟨s, le_trans hsr hrq, x, ℙ.domain_antimonotone hsr hx, H⟩
+  · intro h q hqp
+    rcases h q hqp with ⟨r, hrq, x, hx, H⟩
+    exact ⟨r, hrq, x, hx, r, by rfl, H⟩
+
+lemma monotone {φ : Semiformula L ξ n} :
+    p ⊩[bv|fv] φ → ∀ q ≤ p, q ⊩[bv|fv] φ := fun h ↦ Forces.monotone h
+
+lemma genricity {n} {bv : Fin n → ℙ.Name} {fv : ξ → ℙ.Name} {φ : Semiformula L ξ n} :
+    (∀ q ≤ p, ∃ r ≤ q, r ⊩[bv|fv] φ) → p ⊩[bv|fv] φ :=
+  match φ with
+  | .rel R v => by
+    suffices
+      (∀ q ≤ p, ∃ r ≤ q, ∀ q ≤ r, ∃ s ≤ q, ℙ.Rel s R fun i ↦ (v i).relationalVal bv fv) →
+      (∀ q ≤ p, ∃ r ≤ q, ℙ.Rel r R fun i ↦ (v i).relationalVal bv fv) by simpa
+    intro h q hqp
+    rcases h q hqp with ⟨r, hrq, H⟩
+    rcases H r (by rfl) with ⟨s, hsr, Hs⟩
+    exact ⟨s, le_trans hsr hrq, Hs⟩
+  | .nrel R v => by
+    suffices
+      (∀ q ≤ p, ∃ r ≤ q, ∀ s ≤ r, ¬ℙ.Rel s R fun i ↦ (v i).relationalVal bv fv) →
+      (∀ q ≤ p, ¬ℙ.Rel q R fun i ↦ (v i).relationalVal bv fv) by simpa
+    intro h q hqp hR
+    rcases h q hqp with ⟨r, hrq, Hr⟩
+    exact Hr r (by rfl) (ℙ.rel_monotone hR r hrq)
+  | ⊤ => by simp
+  | ⊥ => by simp
+  | φ ⋏ ψ => by
+    suffices (∀ q ≤ p, ∃ r ≤ q, r ⊩[bv|fv] φ ∧ r ⊩[bv|fv] ψ) → p ⊩[bv|fv] φ ∧ p ⊩[bv|fv] ψ by simpa
+    intro h
+    refine ⟨genricity fun q hqp ↦ ?_, genricity fun q hqp ↦ ?_⟩
+    · rcases h q hqp with ⟨r, hrq, h, _⟩
+      exact ⟨r, hrq, h⟩
+    · rcases h q hqp with ⟨r, hrq, _, h⟩
+      exact ⟨r, hrq, h⟩
+  | φ ⋎ ψ => by
+    suffices
+      (∀ q ≤ p, ∃ r ≤ q, ∀ q ≤ r, ∃ r ≤ q, r ⊩[bv|fv] φ ∨ r ⊩[bv|fv] ψ) →
+      (∀ q ≤ p, ∃ r ≤ q, r ⊩[bv|fv] φ ∨ r ⊩[bv|fv] ψ) by simpa
+    intro h q hqp
+    rcases h q hqp with ⟨r, hrq, H⟩
+    rcases H r (by rfl) with ⟨s, hsr, Hs⟩
+    exact ⟨s, le_trans hsr hrq, Hs⟩
+  | ∀' φ => by
+    suffices
+      (∀ q ≤ p, ∃ r ≤ q, ∀ q ≤ r, ∀ a ∈ ℙ.Domain q, q ⊩[a :> bv|fv] φ) →
+      (∀ q ≤ p, ∀ x ∈ ℙ.Domain q, q ⊩[x :> bv|fv] φ) by simpa
+    intro h q hqp x hx
+    apply genricity
+    intro r hrq
+    rcases h r (le_trans hrq hqp) with ⟨s, hsr, Hs⟩
+    exact ⟨s, hsr, Hs s (by rfl) x (ℙ.domain_antimonotone' hx _ (le_trans hsr hrq))⟩
+  | ∃' φ => by
+    suffices
+      (∀ q ≤ p, ∃ r ≤ q, ∀ q ≤ r, ∃ r ≤ q, ∃ x ∈ ℙ.Domain r, r ⊩[x :> bv|fv] φ) →
+      (∀ q ≤ p, ∃ r ≤ q, ∃ x ∈ ℙ.Domain r, r ⊩[x :> bv|fv] φ) by simpa
+    intro h q hqp
+    rcases h q hqp with ⟨r, hrq, H⟩
+    rcases H r (by rfl) with ⟨s, hsr, x, hx, H⟩
+    exact ⟨s, le_trans hsr hrq, x, hx, H⟩
+
+lemma genricity_iff {φ : Semiformula L ξ n} :
+    p ⊩[bv|fv] φ ↔ ∀ q ≤ p, ∃ r ≤ q, r ⊩[bv|fv] φ :=
+  ⟨fun H q hqp ↦ ⟨q, by rfl, H.monotone q hqp⟩, genricity⟩
+
+lemma genricity_iff_not {φ : Semiformula L ξ n} :
+    ¬p ⊩[bv|fv] φ ↔ ∃ q ≤ p, ∀ r ≤ q, ¬r ⊩[bv|fv] φ := by simpa using genricity_iff.not
+
+@[simp] lemma not {n} {bv : Fin n → ℙ.Name} {fv : ξ → ℙ.Name} {φ : Semiformula L ξ n} :
+    p ⊩[bv|fv] ∼φ ↔ ∀ q ≤ p, ¬q ⊩[bv|fv] φ :=
+  match φ with
+  | .rel R v => by
+    suffices
+      (∀ q ≤ p, ¬ℙ.Rel q R fun i ↦ (v i).relationalVal bv fv) ↔
+      (∀ q ≤ p, ∃ r ≤ q, ∀ s ≤ r, ¬ℙ.Rel s R fun i ↦ (v i).relationalVal bv fv) by simpa
+    constructor
+    · intro h q hqp
+      exact ⟨q, by rfl, fun r hrq ↦ h r (le_trans hrq hqp)⟩
+    · intro h q hqp H
+      rcases h q hqp with ⟨r, hrq, Hr⟩
+      exact Hr r (by rfl) (ℙ.rel_monotone H _ hrq)
+  | .nrel R v => by simp
+  | ⊤ => by simp
+  | ⊥ => by simp
+  | φ ⋏ ψ => by
+    suffices
+        (∀ q ≤ p, ∃ r ≤ q, r ⊩[bv|fv] ∼φ ∨ r ⊩[bv|fv] ∼ψ) ↔
+        (∀ q ≤ p, ¬q ⊩[bv|fv] φ ∨ ¬q ⊩[bv|fv] ψ) by
+      simpa [-not_and, not_and_or]
+    constructor
+    · intro h q hqp
+      rcases h q hqp with ⟨r, hrq, (H | H)⟩
+      · left; intro Hqφ
+        exact WeaklyForces.not.mp H r (by rfl) (Hqφ.monotone _ hrq)
+      · right; intro Hqψ
+        exact WeaklyForces.not.mp H r (by rfl) (Hqψ.monotone _ hrq)
+    · intro h q hqp
+      rcases h q hqp with (C | C)
+      · rcases genricity_iff_not.mp C with ⟨r, hrq, Hr⟩
+        refine ⟨r, hrq, ?_⟩
+        left; apply WeaklyForces.not.mpr Hr
+      · rcases genricity_iff_not.mp C with ⟨r, hrq, Hr⟩
+        refine ⟨r, hrq, ?_⟩
+        right; apply WeaklyForces.not.mpr Hr
+  | φ ⋎ ψ => by
+    suffices
+      p ⊩[bv|fv] ∼φ ∧ p ⊩[bv|fv] ∼ψ ↔
+      ∀ q ≤ p, ∃ r ≤ q, ∀ s ≤ r, ¬s ⊩[bv|fv] φ ∧ ¬s ⊩[bv|fv] ψ by simpa
+    constructor
+    · intro h q hqp
+      refine ⟨q, by rfl, fun r hrq ↦ ⟨?_, ?_⟩⟩
+      · exact WeaklyForces.not.mp h.1 r (le_trans hrq hqp)
+      · exact WeaklyForces.not.mp h.2 r (le_trans hrq hqp)
+    · intro h
+      constructor
+      · apply WeaklyForces.not.mpr
+        intro q hqp Hq
+        rcases h q hqp with ⟨r, hrq, H⟩
+        exact (H r (by rfl)).1 (Hq.monotone _ hrq)
+      · apply WeaklyForces.not.mpr
+        intro q hqp Hq
+        rcases h q hqp with ⟨r, hrq, H⟩
+        exact (H r (by rfl)).2 (Hq.monotone _ hrq)
+  | ∀' φ => by
+    suffices
+      (∀ q ≤ p, ∃ r ≤ q, ∃ a ∈ ℙ.Domain r, r ⊩[a :> bv|fv] ∼φ) ↔
+      (∀ q ≤ p, ∃ r ≤ q, ∃ x ∈ ℙ.Domain r, ¬r ⊩[x :> bv|fv] φ) by simpa
+    constructor
+    · intro h q hqp
+      rcases h q hqp with ⟨r, hrq, x, hx, Hr⟩
+      exact ⟨r, hrq, x, hx, WeaklyForces.not.mp Hr r (by rfl)⟩
+    · intro h q hqp
+      rcases h q hqp with ⟨r, hrq, x, hx, H⟩
+      rcases genricity_iff_not.mp H with ⟨s, hsr, Hs⟩
+      exact ⟨s, le_trans hsr hrq, x, ℙ.domain_antimonotone hsr hx, WeaklyForces.not.mpr Hs⟩
+  | ∃' φ => by
+    suffices
+      (∀ q ≤ p, ∀ a ∈ ℙ.Domain q, q ⊩[a :> bv|fv] ∼φ) ↔
+      (∀ q ≤ p, ∃ r ≤ q, ∀ s ≤ r, ∀ x ∈ ℙ.Domain s, ¬s ⊩[x :> bv|fv] φ) by simpa
+    constructor
+    · intro h q hqp
+      refine ⟨q, by rfl, ?_⟩
+      intro r hrq x hx
+      exact WeaklyForces.not.mp (h r (le_trans hrq hqp) x hx) r (by rfl)
+    · intro h q hqp x hx
+      apply WeaklyForces.not.mpr
+      intro r hrq Hr
+      rcases h r (le_trans hrq hqp) with ⟨s, hsr, H⟩
+      have : ¬s ⊩[x :> bv|fv] φ := H s (by rfl) x (ℙ.domain_antimonotone (le_trans hsr hrq) hx)
+      exact this (Hr.monotone _ hsr)
+
+lemma genricity_iff_not' {φ : Semiformula L ξ n} :
+    ¬p ⊩[bv|fv] φ ↔ ∃ q ≤ p, q ⊩[bv|fv] ∼φ := by simpa using genricity_iff.not
+
+@[simp] lemma imply {φ ψ : Semiformula L ξ n} :
+    p ⊩[bv|fv] φ ➝ ψ ↔ ∀ q ≤ p, q ⊩[bv|fv] φ → q ⊩[bv|fv] ψ := by
+  suffices
+    (∀ q ≤ p, ∃ r ≤ q, (∀ q ≤ r, ¬q ⊩[bv|fv] φ) ∨ r ⊩[bv|fv] ψ) ↔
+    (∀ q ≤ p, q ⊩[bv|fv] φ → q ⊩[bv|fv] ψ) by simpa [DeMorgan.imply]
+  constructor
+  · intro h q hqp Hqφ
+    by_contra! Hqψ
+    rcases genricity_iff_not.mp Hqψ with ⟨r, hrq, Hr⟩
+    rcases h r (le_trans hrq hqp) with ⟨s, hsr, (H | H)⟩
+    · exact H s (by rfl) (Hqφ.monotone s (le_trans hsr hrq))
+    · exact Hr s hsr H
+  · intro h q hqp
+    have : ¬q ⊩[bv|fv] φ ∨ q ⊩[bv|fv] ψ := not_or_of_imp (h q hqp)
+    rcases this with (H | H)
+    · rcases genricity_iff_not.mp H with ⟨r, hrq, H⟩
+      exact ⟨r, hrq, Or.inl H⟩
+    · exact ⟨q, by rfl, Or.inr H⟩
+
+@[simp] lemma iff {φ ψ : Semiformula L ξ n} :
+    p ⊩[bv|fv] φ ⭤ ψ ↔ ∀ q ≤ p, q ⊩[bv|fv] φ ↔ q ⊩[bv|fv] ψ := by
+  simp [LogicalConnective.iff]; grind
+
+end WeaklyForces
+
+abbrev WeaklyForces₀ (p : ℙ) (φ : Sentence L) : Prop := p ⊩[![]|Empty.elim] ↑φ
+
+instance : WeakForcingRelation ℙ (Sentence L) := ⟨WeaklyForces₀⟩
+
+lemma weaklyForces₀_def {p : ℙ} {φ : Sentence L} : p ⊩ᶜ φ ↔ p ⊩[![]|Empty.elim] φ := by rfl
+
+lemma weaklyForces₀_iff_forces {p : ℙ} {φ : Sentence L} :
+    p ⊩ᶜ φ ↔ p ⊩ φᴺ := by rfl
+
+namespace WeaklyForces₀
+
+lemma monotone {p : ℙ} : p ⊩ᶜ φ → ∀ q ≤ p, q ⊩ᶜ φ := WeaklyForces.monotone
+
+lemma genericity {p : ℙ} :
+    (∀ q ≤ p, ∃ r ≤ q, r ⊩ᶜ φ) → p ⊩ᶜ φ := WeaklyForces.genricity
+
+lemma genericity_iff {p : ℙ} :
+    p ⊩ᶜ φ ↔ ∀ q ≤ p, ∃ r ≤ q, r ⊩ᶜ φ := WeaklyForces.genricity_iff
+
+instance : WeakForcingRelation.ClassicalKripke ℙ (· ≥ ·) where
+  verum w := by simp [weaklyForces₀_def]
+  falsum w := by simp [weaklyForces₀_def, WeakForcingRelation.NotForces]
+  and w := by simp [weaklyForces₀_def]
+  or w := by simp [weaklyForces₀_def]
+  imply w := by simp [weaklyForces₀_def]
+  not w := by simp [weaklyForces₀_def, WeakForcingRelation.NotForces]
+
+end WeaklyForces₀
+
+end KripkeModel
